Better error messages and support for let declarations
Put parser into an expection monad to get better error messages.
This results in extremely long compilation and extraction times,
for reasons I'm not particularly sure of. Explicitly giving the
typeclass instances to use could help?

src/Parse.v
@@ -6,6 +6,9 @@ Require Import Ascii.
 Require Import Bool.
 Require Import ExtLib.Data.Strings.
 Require Import ExtLib.Core.RelDec.
+Require Import ExtLib.Structures.Monads.
+Require Import ExtLib.Data.Monads.EitherMonad.
+Require Import ExtLib.Programming.Show.
 Require Import Program.
 Require Import Omega.
 Require Import Wf.
@@ -39,10 +42,46 @@ Set Strict Implicit.
 *)
 Module Parse.
   Import Lambda.
+
+Section monadic.
+  Import MonadNotation.
+  Local Open Scope monad_scope.
+
+  Variable m : Type -> Type.
+  Context {Monad_m : Monad m}.
+  Context {MonadExc_m : MonadExc string m}.
+
   (** Lexing *)
   Inductive token :=
-    LPAREN | RPAREN | AT | QUOTE | COMMA | LAMBDA | LAMBDAS | LETREC
+    LPAREN | RPAREN | AT | QUOTE | COMMA | LAMBDA | LAMBDAS | LETREC | LET
   | DEFINE | MATCH | ID : string -> token.
+
+  Section Printing.
+    Import ShowNotation.
+    Local Open Scope string_scope.
+    Local Open Scope show_scope.
+
+    Global Instance Show_token : Show token :=
+      fun t =>
+        match t with
+          | LPAREN => "("
+          | RPAREN => ")"
+          | AT => "@"
+          | QUOTE => "`"
+          | COMMA => ","
+          | LAMBDA => "lambda"
+          | LAMBDAS => "lambdas"
+          | LETREC => "letrec"
+          | LET => "let"  
+          | DEFINE => "define"
+          | MATCH => "match"
+          | ID s => s ++ " "
+        end.
+
+    Global Instance Show_tokens : Show (list token) :=
+      fun ts => iter_show (map show ts).
+
+  End Printing.
 
   Fixpoint list2string (cs:list ascii) : string :=
     match cs with
@@ -74,6 +113,7 @@ Module Parse.
     ("lambda",LAMBDA)::
     ("lambdas",LAMBDAS)::
     ("letrec",LETREC)::
+    ("let",LET)::
     ("define",DEFINE)::
     ("match",MATCH)::
     nil.
@@ -148,198 +188,229 @@ Module Parse.
   End TOKENIZE.
 
   (** Parsing *)
-  Fixpoint parse (ts:list token) (fuel:nat) : option (list (var * exp)) :=
+  Fixpoint parse (ts:list token) (fuel:nat) : m (list (var * exp)) :=
     match fuel with
-      | O => None
+      | O => raise "Ran out of fuel during parse"
       | S fuel =>
         match ts with
-          | nil => Some nil
+          | nil => ret nil
           | LPAREN::DEFINE::(ID x)::ts1 =>
-            match parse_exp' ts1 fuel with
-              | Some (e,RPAREN::ts2) =>
-                match parse ts2 fuel with
-                  | Some es => Some ((Env.wrapVar x,e)::es)
-                  | _ => None
-                end
-              | _ => None
+            res <- parse_exp' ts1 fuel ;;
+            match res with
+              | (e,RPAREN::ts2) =>
+                es <- parse ts2 fuel ;;
+                ret ((Env.wrapVar x,e)::es)
+              | _ => raise "Parse error while parsing define"
             end
-          | _ => None
+          | _ => raise "Parse error while parsing definitions"
         end
     end
-  with parse_exp' (ts:list token) (fuel:nat) : option (exp * (list token)) :=
+  with parse_exp' (ts:list token) (fuel:nat) : m (exp * (list token)) :=
     match fuel with
-      | O => None
+      | O => raise "Ran out of fuel during parse_exp'"
       | S fuel =>
         match ts with
         (* EXP -> <ID> *)
-          | (ID x)::ts2 => Some (Var_e (Env.wrapVar x), ts2)
+          | (ID x)::ts2 => ret (Var_e (Env.wrapVar x), ts2)
         (* EXP -> (lambda (<ID>) <EXP>) *)
           | LPAREN::LAMBDA::LPAREN::(ID x)::RPAREN::ts2 =>
-            match parse_exp' ts2 fuel with
-              | Some (e,RPAREN::ts3) => Some (Lam_e (Env.wrapVar x) e,ts3)
-              | _ => None
+            res <- parse_exp' ts2 fuel ;;
+            match res with
+              | (e,RPAREN::ts3) => ret (Lam_e (Env.wrapVar x) e,ts3)
+              | _ => raise "Error parsing lambda, expecting expression"
             end
           (* EXP -> (lambdas (<ARGLIST>) <EXP>) *)
           | LPAREN::LAMBDAS::LPAREN::ts2 =>
-            match parse_arglist ts2 fuel with
-              | Some (xs,RPAREN::ts3) =>
-                match parse_exp' ts3 fuel with
-                  | Some (e,RPAREN::ts4) =>
-                    Some (fold_right Lam_e e xs,ts4)
-                  | _ => None
+            res <- parse_arglist ts2 fuel ;;
+            match res with
+              | (xs,RPAREN::ts3) =>
+                res <- parse_exp' ts3 fuel ;;
+                match res with
+                  | (e,RPAREN::ts4) =>
+                    ret (fold_right Lam_e e xs,ts4)
+                  | _ => raise "Error parsing lambda, expecting expression"
                 end
-              | _ => None
+              | _ => raise "Error parsing lambda, expecting arguments"
             end
           (* EXP -> `(<ID> <CONARGLIST>) *)
           | QUOTE::LPAREN::(ID c)::ts2 =>
-            match parse_conarglist ts2 fuel with
-              | Some (es,RPAREN::ts3) =>
-                Some (Con_e c es,ts3)
-              | _ => None
+            res <- parse_conarglist ts2 fuel ;;
+            match res with
+              | (es,RPAREN::ts3) =>
+                ret (Con_e c es,ts3)
+              | _ => raise "Error parsing constructor"
             end
           (* EXP -> (@ <EXPLIST>) *)
           | LPAREN::AT::ts2 =>
-            match parse_exp' ts2 fuel with
-              | Some (e1,ts3) =>
-                match parse_exp'list ts3 fuel with
-                  | Some (es,RPAREN::ts4) =>
-                    Some (fold_left App_e es e1,ts4)
-                  | _ => None
+            res <- parse_exp' ts2 fuel ;;
+            match res with
+              | (e1,ts3) =>
+                res <- parse_exp'list ts3 fuel ;;
+                match res with
+                  | (es,RPAREN::ts4) =>
+                    ret (fold_left App_e es e1,ts4)
+                  | _ => raise "Error parsing unquote, expecting expression list"
                 end
-              | _ => None
             end
           (* EXP -> (match <EXP> <ARMLIST>) *)
           | LPAREN::MATCH::ts1 =>
-            match parse_exp' ts1 fuel with
-              | Some (e,ts2) =>
-                match parse_armlist ts2 fuel with
-                  | Some (arms,RPAREN::ts3) =>
-                    Some (Match_e e arms,ts3)
-                  | _ => None
+            res <- parse_exp' ts1 fuel ;;
+            match res with
+              | (e,ts2) =>
+                res <- parse_armlist ts2 fuel ;;
+                match res with
+                  | (arms,RPAREN::ts3) =>
+                    ret (Match_e e arms,ts3)
+                  | _ => raise "Error parsing match, expecting arm list"
                 end
-              | _ => None
             end
           (* EXP -> (letrec (<DECLLIST>) <EXP>) *)
           | LPAREN::LETREC::LPAREN::ts1 =>
-            match parse_decllist ts1 fuel with
-              | Some (ds,RPAREN::ts2)=>
-                match parse_exp' ts2 fuel with
-                  | Some (e,RPAREN::ts3) =>
-                    Some (Letrec_e ds e,ts3)
-                  | _ => None
+            res <- parse_decllist ts1 fuel ;;
+            match res with
+              | (ds,RPAREN::ts2) =>
+                res <- parse_exp' ts2 fuel ;;
+                match res with
+                  | (e,RPAREN::ts3) =>
+                    ret (Letrec_e ds e,ts3)
+                  | _ => raise "Error parsing letrec, expecting expression"
                 end
-              | _ => None
+              | _ => raise "Error parsing letrec, expecting declaration list"
+            end
+          (* EXP -> (let (<DECL>) <EXP>) *)
+          | LPAREN::LET::LPAREN::ts1 =>
+            res <- parse_decl ts1 fuel ;;
+            match res with
+              | ((v,d),RPAREN::ts2) =>
+                res <- parse_exp' ts2 fuel ;;
+                match res with
+                  | (e,RPAREN::ts3) =>
+                    ret (Let_e v d e,ts3)
+                  | _ => raise "Error parsing let, expecting expression"
+                end
+              | _ => raise "Error parsing let, expecting declaration"
             end
           (* EXP -> (<EXP> <EXP>) *)
           | LPAREN::ts2 =>
-            match parse_exp' ts2 fuel with
-              | Some (e1,ts3) =>
-                match parse_exp' ts3 fuel with
-                  | Some (e2,RPAREN::ts4) =>
-                    Some (App_e e1 e2,ts4)
-                  | _ => None
+            res <- parse_exp' ts2 fuel ;;
+            match res with
+              | (e1,ts3) =>
+                res <- parse_exp' ts3 fuel ;;
+                match res with
+                  | (e2,RPAREN::ts4) =>
+                    ret (App_e e1 e2,ts4)
+                  | _ => raise "Error parsing application, expecting expression"
                 end
-              | _ => None
             end
-          | _ => None
+          | t::ts => raise ("Error parsing expression, unexpected token " ++ (to_string t) ++ " while trying to parse " ++ to_string (t::ts))%string
+          | nil => raise "Error parsing expression, unexpected EOF"
         end
     end
 
-  with parse_exp'list (ts:list token) (fuel:nat) : option ((list exp) * (list token)) :=
+  with parse_exp'list (ts:list token) (fuel:nat) : m ((list exp) * (list token)) :=
     match fuel with
-      | O => None
+      | O => raise "Ran out of fuel during parse_exp'list"
       | S fuel =>
-        match parse_exp' ts fuel with
-          | Some (e,ts2) =>
-            match parse_exp'list ts2 fuel with
-              | Some (es,ts3) => Some (e::es,ts3)
-              | None => None
-            end
-          | None => Some (nil,ts)
-        end
+        res <- parse_exp' ts fuel ;;
+        let '(e,ts2) := res in
+        res <- parse_exp'list ts2 fuel ;;
+        let '(es,ts3) := res in
+        ret (e::es,ts3)
     end
 
-  with parse_conarglist (ts:list token) (fuel:nat) : option ((list exp) * (list token)) :=
+  with parse_conarglist (ts:list token) (fuel:nat) : m ((list exp) * (list token)) :=
     match fuel with
-      | O => None
+      | O => raise "Ran out of fuel during parse_conarglist"
       | S fuel =>
         match ts with
           | COMMA::ts1 =>
-            match parse_exp' ts1 fuel with
-              | Some (e,ts2) =>
-                match parse_conarglist ts2 fuel with
-                  | Some (es,ts3) => Some (e::es,ts3)
-                  | None => None
-                end
-              | None => None
-            end
-          | _ => Some (nil,ts)
+            res <- parse_exp' ts1 fuel ;;
+            let '(e,ts2) := res in
+            res <- parse_conarglist ts2 fuel ;;
+            let '(es,ts3) := res in
+            ret (e::es,ts3)
+          | _ => ret (nil,ts)
         end
     end
 
-  with parse_arglist (ts:list token) (fuel:nat) : option ((list var) * (list token)) :=
+  with parse_arglist (ts:list token) (fuel:nat) : m ((list var) * (list token)) :=
     match fuel with
-      | O => None
+      | O => raise "Ran out of fuel during parse_arglist"
       | S fuel =>
       (* ARGLIST -> <ID> <ARGLIST> | epsilon *)
         match ts with
           | (ID x)::ts2 =>
-            match parse_arglist ts2 fuel with
-              | Some (xs,ts3) =>
-                Some (Env.wrapVar x::xs,ts3)
-              | _ => None
-            end
-          | _ => Some (nil,ts)
+            res <- parse_arglist ts2 fuel ;;
+            let '(xs,ts3) := res in
+            ret (Env.wrapVar x::xs,ts3)
+          | _ => ret (nil,ts)
         end
     end
 
-  with parse_armlist (ts:list token) (fuel:nat) : option ((list (pattern*exp)) * (list token)) :=
+  with parse_armlist (ts:list token) (fuel:nat) : m ((list (pattern*exp)) * (list token)) :=
     match fuel with
-      | O => None
+      | O => raise "Ran out of fuel during parse_armlist"
       | S fuel =>
       (* ARMLIST -> ((<ID> <ARGLIST>) <EXP>) ARMLIST | epsilon *)
         match ts with
           | LPAREN::LPAREN::(ID c)::ts1 =>
-            match parse_arglist ts1 fuel with
-              | Some (xs,RPAREN::ts2) =>
-                match parse_exp' ts2 fuel with
-                  | Some (e,RPAREN::ts3) =>
-                    match parse_armlist ts3 fuel with
-                      | Some (arms,ts4) =>
-                        Some ((Con_p c xs,e)::arms,ts4)
-                      | _ => None
-                    end
-                  | _ => None
+            res <- parse_arglist ts1 fuel ;;
+            match res with
+              | (xs,RPAREN::ts2) =>
+                res <- parse_exp' ts2 fuel ;;
+                match res with
+                  | (e,RPAREN::ts3) =>
+                    res <- parse_armlist ts3 fuel ;;
+                    let '(arms,ts4) := res in
+                    ret ((Con_p c xs,e)::arms,ts4)
+                  | _ => raise "Error parsing arm list"
                 end
-              | _ => None
+              | _ => raise "Error parsing arm list"
             end
-          | _ => Some (nil,ts)
+          | _ => ret (nil,ts)
         end
     end
 
-  with parse_decllist (ts:list token) (fuel:nat) : option ((list (var*(var*exp))) * (list token)) :=
+  with parse_decl (ts:list token) (fuel:nat) : m ((var * exp) * (list token)) :=
     match fuel with
-      | O => None
+      | O => raise "Ran out of fuel during parse_decl"
+      | S fuel =>
+        match ts with
+          | LPAREN::(ID v)::ts1 =>
+            res <- parse_exp' ts1 fuel ;;
+            match res with
+              | (e,RPAREN::ts2) =>
+                ret ((Env.wrapVar v,e),ts2)
+              | _ => raise "Error parsing declaration, expecting expression"
+            end
+          | _ => raise "Error parsing declaration, expecting id"
+        end 
+    end
+
+  with parse_decllist (ts:list token) (fuel:nat) : m ((list (var*(var*exp))) * (list token)) :=
+    match fuel with
+      | O => raise "Ran out of fuel during parse_decllist"
       | S fuel =>
         match ts with
           | LPAREN::(ID f)::ts1 =>
-            match parse_exp' ts1 fuel with
-              | Some (Lam_e x e,RPAREN::ts2) =>
-                match parse_decllist ts2 fuel with
-                  | Some (ds,ts3) =>
-                    Some ((Env.wrapVar f,(x,e))::ds,ts3)
-                  | _ => None
-                end
-              | _ => None
+            res <- parse_exp' ts1 fuel ;;
+            match res with
+              | (Lam_e x e,RPAREN::ts2) =>
+                res <- parse_decllist ts2 fuel ;;
+                let '(ds,ts3) := res in
+                ret ((Env.wrapVar f,(x,e))::ds,ts3)
+              | _ => raise "Error parsing declaration list, expecting lambda term"
             end
-          | _ => Some (nil,ts)
+          | _ => ret (nil,ts)
         end
     end.
 
+End monadic.
+
   (** A parser for expresions *)
-  Definition parse_exp (s:string) : option (exp * list token) :=
+  Definition parse_exp (s:string) : string + (exp * list token) :=
     match tokenize s nil with
-      | None => None
+      | None => inl "Parse error: tokenizer failed"%string
       | Some ts => parse_exp' ts (List.length ts) 
     end.
 
@@ -382,24 +453,23 @@ Module Parse.
       | _ :: ds => lastDecl ds
     end.
     
-
   (** Parse a set of top-level declarations and return a bit "let", binding
       those declarations, terminated by a call to "main tt".  Of course, this
       is only meaningful if one of the declarations binds a function that takes
       unit as an argument... *)
-  Definition parse_topdecls (s:string) : option exp :=
+  Definition parse_topdecls (s:string) : string + exp :=
     match tokenize s nil with
-      | None => None
+      | None => inl "Parse error: tokenizer failed"%string
       | Some ts => match parse ts (List.length ts) with
-                     | None => None
-                     | Some ds =>
+                     | inl e => inl e
+                     | inr ds =>
                        let body := 
                          match lastDecl ds with
-                           | None => Con_e "Tt" nil
-                           | Some v => Var_e v 
+                           | None => Con_e "Tt"%string nil
+                           | Some v => Var_e v
                            end
                        in
-                       Some (collapse_decls ds nil body)
+                       inr (collapse_decls ds nil body)
                    end
     end.
 
